src/lib/GPU.Seq.Common.fsti
@@ -29,3 +29,7 @@ val lemma_seq_fold_left_sum (#a:Type) (e:a) (f: a -> a -> a)
   : Lemma (requires is_monoid e f)
           (ensures seq_fold_left f e (append s1 s2)
                    == f (seq_fold_left f e s1) (seq_fold_left f e s2))
+
+val lem_append_slice (#a:Type) (s : seq a) (i j k : nat)
+  : Lemma (requires i <= j /\ j <= k /\ k <= length s)
+          (ensures append (slice s i j) (slice s j k) == slice s i k)
